feat: Primcodable.wtype

Logic/Vorspiel/Computability.lean
@@ -1,7 +1,5 @@
 import Logic.Vorspiel.Vorspiel
 
-variable {α : Type u}
-
 namespace Nat
 
 def predO : ℕ → Option ℕ
@@ -20,7 +18,56 @@ def range2 (n m : ℕ) : List (ℕ × ℕ) := (·, ·) <$> range n <*> range m
 
 @[simp] lemma mem_range2_iff {n m i j : ℕ} : (i, j) ∈ range2 n m ↔ i < n ∧ j < m := by simp[range2, seq_eq_bind]
 
+def toVector (n : ℕ) : List α → Option (Vector α n) := fun l => if h : l.length = n then some ⟨l, h⟩ else none
+
 end List
+
+namespace Encodable
+
+variable {ι : Type _} [Fintype ι] [DecidableEq ι] [Encodable ι]
+
+def fintypeArrowEquivFinArrow : (ι → α) ≃ (Fin (Fintype.card ι) → α) :=
+  Equiv.arrowCongr fintypeEquivFin (Equiv.refl α)
+
+def fintypeArrowEquivVector : (ι → α) ≃ (Vector α (Fintype.card ι)) :=
+  fintypeArrowEquivFinArrow.trans (Equiv.vectorEquivFin α (Fintype.card ι)).symm
+
+lemma fintypeArrowEquivFinArrow_eq (f : ι → α) : fintypeArrowEquivFinArrow f = fun i => f (fintypeEquivFin.symm i) := by rfl
+
+@[simp] lemma fintypeArrowEquivFinArrow_app (f : ι → α) (i) : fintypeArrowEquivFinArrow f i = f (fintypeEquivFin.symm i) := by rfl
+
+@[simp] lemma fintypeArrowEquivFinArrow_symm_app (v : Fin (Fintype.card ι) → α) :
+    fintypeArrowEquivFinArrow.symm v i = v (fintypeEquivFin i) := by rfl
+
+@[simp] lemma fintypeArrowEquivVector_app (f : ι → α) : (fintypeArrowEquivVector f).get i = f (fintypeEquivFin.symm i) := by
+  simp[fintypeArrowEquivVector, Equiv.vectorEquivFin]
+
+@[simp] lemma fintypeArrowEquivVector_symm_app (v : Vector α (Fintype.card ι)) :
+    (fintypeArrowEquivVector.symm v) i = v.get ((fintypeEquivFin i)) := by rfl
+
+@[simp] lemma fintypeArrowEquivFinArrow_fintypeEquivFin (f : Fin (Fintype.card ι) → α) :
+    fintypeArrowEquivFinArrow (fun i => f (fintypeEquivFin i)) = f := by funext i; simp
+
+def toFinArrowOpt (f : ι → Option α) : Option (ι → α) :=
+  (Matrix.toOptionVec (fintypeArrowEquivFinArrow f)).map fintypeArrowEquivFinArrow.symm
+
+@[simp] lemma toFinArrowOpt_eq_none_iff {f : ι → Option α} : toFinArrowOpt f = none ↔ ∃ i, f i = none := by
+  simp[toFinArrowOpt, fintypeArrowEquivFinArrow]; constructor
+  { rintro ⟨i, hi⟩; exact ⟨_, hi⟩ }; { rintro ⟨i, hi⟩; exact ⟨fintypeEquivFin i, by simp[hi]⟩  }
+
+@[simp] lemma toFinArrowOpt_eq_some_iff {f : ι → Option α} {g} : toFinArrowOpt f = some g ↔ ∀ i, f i = some (g i) := by
+  simp[toFinArrowOpt, fintypeArrowEquivFinArrow]; constructor
+  { rintro ⟨a, ha, rfl⟩; simp; intro i
+    simpa using ha (fintypeEquivFin i) }
+  { intro hf; exact ⟨fun i => g (fintypeEquivFin.symm i), by { simp[hf]; funext i; simp }⟩ }
+
+@[simp] lemma vectorEquivFin_symm_val (f : Fin n → β) : ((Equiv.vectorEquivFin β n).symm f).toList = List.ofFn f := by
+  ext i b; simp[Equiv.vectorEquivFin, Vector.ofFn]
+
+-- todo: move to Vorspiel
+@[simp] def getI_ofFn [Inhabited α] {n} (f : Fin n → α) (i : Fin n) : (List.ofFn f).getI i = f i := by simp[List.getI_eq_get]
+
+end Encodable
 
 namespace Encodable
 
@@ -31,6 +78,9 @@ variable {α : Type _} [Encodable α]
 lemma encodeDecode_of_none {e : ℕ} (h : decode (α := α) e = none) : encodeDecode α e = none := by simp[encodeDecode, h]
 
 lemma encodeDecode_of_some {e : ℕ} {a : α} (h : decode e = some a) : encodeDecode α e = some (encode a) := by simp[encodeDecode, h]
+
+lemma encodeDecode_eq_encode_map_decode {e : ℕ} : encodeDecode α e = (decode e : Option α).map encode := by
+  simp[encodeDecode]; rcases (decode e) <;> simp
 
 lemma decode_encodeDecode : encodeDecode α e = some i → ∃ a : α, decode i = some a := by
   simp[encodeDecode]
@@ -55,22 +105,7 @@ lemma encodeDecode_subtype (e : ℕ) :
   simp[encodeDecode_subtype', encodeDecode]
   rcases (decode e : Option α) <;> simp
 
--- todo: delete
-lemma encode_decode_ofEquiv {β} (e : β ≃ α) (n : ℕ) :
-    haveI : Encodable β := Encodable.ofEquiv α e
-    encode (decode (α := β) n) = encode (decode (α := α) n) := by
-  simp[Encodable.decode_ofEquiv e]
-  rcases h : (decode n : Option α) with (_ | ⟨a⟩) <;> simp
-  { exact @Encodable.encode_none _ (Encodable.ofEquiv α e) }
-  { have := @Encodable.encode_some _ (Encodable.ofEquiv α e) (e.symm a); rw[this];
-    simpa using Encodable.encode_ofEquiv e (e.symm a) }
-
--- todo: delete
-lemma encode_decode_ofEquiv_prim {α β} [Primcodable α] (e : β ≃ α) (n : ℕ) :
-    haveI : Primcodable β := Primcodable.ofEquiv α e
-    encode (decode (α := β) n) = encode (decode (α := α) n) := encode_decode_ofEquiv e n
-
-lemma encodeDecode_ofEquiv {β} (e : β ≃ α) :
+lemma encodeDecode_ofEquiv (α) [Encodable α] {β} (e : β ≃ α) :
     haveI : Encodable β := Encodable.ofEquiv α e
     encodeDecode β = encodeDecode α := by
   funext n; simp[encodeDecode, Encodable.decode_ofEquiv e]
@@ -78,6 +113,10 @@ lemma encodeDecode_ofEquiv {β} (e : β ≃ α) :
   { simp[@Encodable.encode_none _ (Encodable.ofEquiv α e)] }
   { have := @Encodable.encode_some _ (Encodable.ofEquiv α e) (e.symm a); rw[this];
     simpa using Encodable.encode_ofEquiv e (e.symm a) } 
+
+lemma encodeDecode_ofEquiv_prim (α) {β} [Primcodable α] (e : β ≃ α) :
+    haveI : Primcodable β := Primcodable.ofEquiv α e
+    encodeDecode β = encodeDecode α := encodeDecode_ofEquiv α e
 
 lemma encode_decode_eq_encodeDecode : encode (decode e : Option α) = encode (encodeDecode α e) := by
   simp[encodeDecode]; cases (decode e : Option α) <;> simp
@@ -101,23 +140,25 @@ namespace Primcodable
 
 open Encodable
 
-instance fintypeArrow [DecidableEq α] [Fintype α] [Encodable α] {β : Type _} [Primcodable β] : Primcodable (α → β) :=
-    Primcodable.ofEquiv (Fin (Fintype.card α) → β) (Equiv.arrowCongr Encodable.fintypeEquivFin (Equiv.refl _))
-
 lemma ofEquiv_toEncodable {α : Type _} {β : Type _} [Primcodable α] (e : β ≃ α) :
   (ofEquiv α e).toEncodable = Encodable.ofEquiv α e := rfl
+
+instance fintypeArrow [DecidableEq α] [Fintype α] [Encodable α] (β : Type _) [Primcodable β] : Primcodable (α → β) :=
+    Primcodable.ofEquiv (Fin (Fintype.card α) → β) fintypeArrowEquivFinArrow
 
 end Primcodable
 
 namespace Primrec
 
-lemma nat_strong_rec' [Primcodable α] [Primcodable σ] (f : α → ℕ → σ) {g : α × ℕ → List σ → Option σ} (hg : Primrec₂ g)
+variable {α : Type _} {β : Type _} {γ : Type _} {σ : Type _} [Primcodable α] [Primcodable β] [Primcodable γ] [Primcodable σ]
+
+lemma nat_strong_rec' (f : α → ℕ → σ) {g : α × ℕ → List σ → Option σ} (hg : Primrec₂ g)
   (H : ∀ a n, g (a, n) ((List.range n).map (f a)) = some (f a n)) : Primrec₂ f := by
   let g' : α → List σ → Option σ := fun a l => g (a, l.length) l
   have : Primrec₂ g' := hg.comp₂ (pair fst (list_length.comp snd)) Primrec₂.right
   exact nat_strong_rec f this (by simpa using H)
 
-lemma nat_strong_rec'2 [Primcodable α] [Primcodable σ] (f : α → ℕ × ℕ → σ) {g : α × (ℕ × ℕ) → List σ → Option σ} (hg : Primrec₂ g)
+lemma nat_strong_rec'2 (f : α → ℕ × ℕ → σ) {g : α × (ℕ × ℕ) → List σ → Option σ} (hg : Primrec₂ g)
   (H : ∀ a n m, g (a, (n, m)) ((List.range (n.pair m)).map (fun i => f a i.unpair)) = some (f a (n, m))) : Primrec₂ f := by
   let g' : α × ℕ → List σ → Option σ := fun (a, n) => g (a, n.unpair)
   have : Primrec₂ g' := hg.comp₂ (pair (fst.comp fst) (unpair.comp $ snd.comp fst)) Primrec₂.right
@@ -126,14 +167,14 @@ lemma nat_strong_rec'2 [Primcodable α] [Primcodable σ] (f : α → ℕ × ℕ 
     this.comp₂ Primrec₂.left (Primrec₂.natPair.comp (fst.comp snd) (snd.comp snd))
   exact this.of_eq (by simp)
 
-lemma nat_strong_rec'2' [Primcodable σ] (f : ℕ → ℕ → σ) {g : ℕ × ℕ → List σ → Option σ} (hg : Primrec₂ g)
+lemma nat_strong_rec'2' (f : ℕ → ℕ → σ) {g : ℕ × ℕ → List σ → Option σ} (hg : Primrec₂ g)
   (H : ∀ n m, g (n, m) ((List.range (n.pair m)).map (fun i => f i.unpair.1 i.unpair.2)) = some (f n m)) : Primrec₂ f := by
   have : Primrec₂ (fun p => g p.2 : Unit × (ℕ × ℕ) → List σ → Option σ) := hg.comp (snd.comp fst) snd
   have := nat_strong_rec'2 (fun _ i => f i.1 i.2 : Unit → ℕ × ℕ → σ) this (by simpa using H)
   have : Primrec₂ (fun n m => (fun _ i => f i.1 i.2 : Unit → ℕ × ℕ → σ) () (n, m)) := this.comp (const ()) Primrec.id
   exact this.of_eq (by simp)
 
-lemma option_list_mapM' [Primcodable α] [Primcodable β] [Primcodable γ]
+lemma option_list_mapM'
   {f : α → List β} {g : α → β → Option γ} (hf : Primrec f) (hg : Primrec₂ g) : Primrec (fun a => (f a).mapM' (g a)) := by
   have : Primrec₂ (fun a p => (g a p.1).bind $ fun c => p.2.2.map $ fun l => c :: l : α → β × List β × Option (List γ) → Option (List γ)) :=
     Primrec.option_bind (hg.comp fst (fst.comp snd)) (Primrec.option_map (snd.comp $ snd.comp $ snd.comp fst) (Primrec.list_cons.comp₂ (snd.comp fst) Primrec₂.right))
@@ -154,23 +195,33 @@ lemma nat_predO : Primrec Nat.predO :=
 
 protected lemma encodeDecode : Primrec (fun e => encodeDecode α e) := nat_predO.comp (Primrec.encode.comp Primrec.decode)
 
-class Uniform {α : Type u} (β : α → Type v) [Primcodable α] [∀ a, Primcodable (β a)] where
+lemma list_sup [SemilatticeSup α] [OrderBot α] (hsup : Primrec₂ (Sup.sup : α → α → α)) : Primrec (List.sup : List α → α) := by
+  have e : ∀ l : List α, l.sup = l.foldr Sup.sup ⊥ := by
+    intro l; induction' l with a as ih <;> simp[sup_eq_max, *]
+  have : Primrec (fun l => l.foldr Sup.sup ⊥ : List α → α) :=
+    list_foldr Primrec.id (const _) (hsup.comp₂ (fst.comp₂ Primrec₂.right) (snd.comp₂ Primrec₂.right))
+  exact this.of_eq (by simp[e])
+
+end Primrec
+
+class UniformlyPrimcodable {α : Type u} (β : α → Type v) [Primcodable α] [(a : α) → Primcodable (β a)] where
   uniformly_prim : Primrec₂ (fun a n => Encodable.encode (Encodable.decode (α := β a) n))
 
-class CardUniform {α : Type u} (β : α → Type v) [∀ a, Fintype (β a)] [Primcodable α] [∀ a, Primcodable (β a)] where
+class PrimrecCard {α : Type u} (β : α → Type v) [∀ a, Fintype (β a)] [Primcodable α] [(a : α) → Primcodable (β a)] where
   card_prim : Primrec fun a => Fintype.card (β a)
 
-namespace Uniform
+namespace UniformlyPrimcodable
 
-variable {α : Type u} {β γ : α → Type v} [Primcodable α] [(a : α) → Primcodable (β a)]
+open Encodable Primcodable Primrec
+variable {α : Type u} {β γ : α → Type v} [Primcodable α] [(a : α) → Primcodable (β a)] [(a : α) → Primcodable (γ a)]
 
-lemma _root_.Primrec₂.encodeDecode_u [Uniform β] : Primrec₂ (fun a e => encodeDecode (β a) e) :=
-  (nat_predO.comp $ Uniform.uniformly_prim.comp fst snd)
+lemma _root_.Primrec₂.encodeDecode_u [UniformlyPrimcodable β] : Primrec₂ (fun a e => encodeDecode (β a) e) :=
+  (nat_predO.comp $ UniformlyPrimcodable.uniformly_prim.comp fst snd)
 
-def ofEncodeDecode (h : Primrec₂ (fun a n => encodeDecode (β a) n)) : Uniform β where
+def ofEncodeDecode (h : Primrec₂ (fun a n => encodeDecode (β a) n)) : UniformlyPrimcodable β where
   uniformly_prim := (Primrec.encode.comp₂ h).of_eq (by simp[encode_decode_eq_encodeDecode])
 
-instance {β : Type _} [Primcodable β] : Uniform (Vector β) where
+instance vector (β : Type _) [Primcodable β] : UniformlyPrimcodable (Vector β) where
   uniformly_prim := by
     have e : ∀ n e, encode ((decode (α := List β) e).bind (fun a => if a.length = n then some a else none)) =
         encode (decode (α := Vector β n) e) := by intro n e; rw[Encodable.encode_decode_subtype]
@@ -183,7 +234,7 @@ instance {β : Type _} [Primcodable β] : Uniform (Vector β) where
 
 attribute [-instance] Encodable.finPi
 
-instance {β : Type _} [Primcodable β] : Uniform (Fin · → β) where
+instance finArrow (β : Type _) [Primcodable β] : UniformlyPrimcodable (Fin · → β) where
   uniformly_prim := by
     have : ∀ n e, encode (decode (α := Vector β n) e) = encode (decode (α := Fin n → β) e) := by
       intro n e; simp[Encodable.decode_ofEquiv]
@@ -193,26 +244,27 @@ instance {β : Type _} [Primcodable β] : Uniform (Fin · → β) where
         simpa using (this (Equiv.vectorEquivFin β n v)).symm }
     exact uniformly_prim.of_eq this
 
-instance fintypeArrow [DecidableEq α] [Fintype α] {β : Type _} [Primcodable β] : Primcodable (α → β) :=
-    Primcodable.ofEquiv (Fin (Fintype.card α) → β) (Equiv.arrowCongr fintypeEquivFin (Equiv.refl _))
-
-instance {γ : α → Type _} [(a : α) → Fintype (γ a)] [(a : α) → DecidableEq (γ a)] [(a : α) → Primcodable (γ a)] [CardUniform γ]
-  {β : Type _} [Primcodable β] : Uniform (γ · → β) where
-  uniformly_prim := by
-    simp[Encodable.encode_decode_ofEquiv_prim]
-    exact (Uniform.uniformly_prim (β := Vector β)).comp₂ (CardUniform.card_prim.comp fst) Primrec₂.right
+instance fintypeArrow (γ : α → Type _) (β : Type _)
+  [(a : α) → Fintype (γ a)] [(a : α) → DecidableEq (γ a)] [(a : α) → Primcodable (γ a)] [PrimrecCard γ] [Primcodable β] :
+    UniformlyPrimcodable (γ · → β) := ofEncodeDecode
+  (by { have : Primrec₂ (fun a n => encodeDecode (Fin (Fintype.card (γ a)) → β) n) :=
+          (Primrec₂.encodeDecode_u (β := (Fin · → β))).comp (PrimrecCard.card_prim.comp fst) snd
+        exact this.of_eq (fun a b =>
+          by { simp[Primcodable.ofEquiv_toEncodable, Encodable.encodeDecode_ofEquiv]
+               rw[Encodable.encodeDecode_ofEquiv (Fin (Fintype.card (γ a)) → β)] }) })
 
 attribute [instance] Encodable.finPi
 
-instance : Uniform Fin where
+instance fin : UniformlyPrimcodable Fin where
   uniformly_prim := by
     have : ∀ e n, encode (decode (α := Fin n) e) = if e < n then e + 1 else 0 := by
       intro e n
       by_cases h : e < n <;> simp[h, Encodable.decode_ofEquiv, decode, decodeSubtype, Encodable.encode_ofEquiv, encode, encodeSubtype]
     exact (Primrec.ite (Primrec.nat_lt.comp snd fst) (Primrec.succ.comp $ snd) (Primrec.const 0)).of_eq (by simp[this])
 
-instance {β : α → Type _} {γ : α → Type _} [(a : α) → Primcodable (β a)] [(a : α) → Primcodable (γ a)] [Uniform β] [Uniform γ] :
-    Uniform (fun a => β a × γ a) where
+instance prod (β : α → Type _) (γ : α → Type _)
+  [(a : α) → Primcodable (β a)] [(a : α) → Primcodable (γ a)] [UniformlyPrimcodable β] [UniformlyPrimcodable γ] :
+    UniformlyPrimcodable (fun a => β a × γ a) where
   uniformly_prim := by
     have e : ∀ a e, encode ((encodeDecode (β a) e.unpair.1).bind $ fun b => (encodeDecode (γ a) e.unpair.2).map $ fun c => Nat.pair b c) =
         encode (decode (α := β a × γ a) e) := by
@@ -229,15 +281,17 @@ instance {β : α → Type _} {γ : α → Type _} [(a : α) → Primcodable (β
             (Primrec₂.natPair.comp₂ (snd.comp $ fst) Primrec₂.right)))
     exact this.of_eq e
 
-instance {β : Type _} [Primcodable β] : Uniform (fun (_ : α) => β) where
+instance const {β : Type _} [Primcodable β] : UniformlyPrimcodable (fun (_ : α) => β) where
   uniformly_prim := (nat_iff.mpr Primcodable.prim).comp snd
 
-end Uniform
+end UniformlyPrimcodable
 
-open Encodable
+namespace Primcodable
+
+open Encodable UniformlyPrimcodable Primrec
 variable {α : Type u} {β : α → Type v} [Primcodable α] [(a : α) → Primcodable (β a)]
 
-instance sigma [Uniform β] : Primcodable (Sigma β) where
+instance sigma [UniformlyPrimcodable β] : Primcodable (Sigma β) where
   prim := by
     have e : ∀ e, encode ((decode e.unpair.1 : Option α).bind (fun a => (encodeDecode (β a) e.unpair.2).map (Nat.pair (encode a)))) =
         encode (decode e : Option (Sigma β)) := by
@@ -252,62 +306,46 @@ instance sigma [Uniform β] : Primcodable (Sigma β) where
         (Primrec₂.natPair.comp₂ (Primrec.encode.comp $ snd.comp $ fst) Primrec₂.right))
     exact Primrec.nat_iff.mp ((Primrec.encode.comp $ p₁.option_bind p₂).of_eq e)
 
-@[simp] lemma sigma_toEncodable_eq [Uniform β] : (sigma : Primcodable (Sigma β)).toEncodable = Sigma.encodable := rfl
+@[simp] lemma sigma_toEncodable_eq [UniformlyPrimcodable β] : (sigma : Primcodable (Sigma β)).toEncodable = Sigma.encodable := rfl
 
-end Primrec
+end Primcodable
 
 namespace Encodable
 
-open Primcodable Primrec.Uniform
+open Primcodable Primrec UniformlyPrimcodable
+variable {β : Type _} [Encodable β]
 attribute [-instance] Encodable.finPi Encodable.fintypeArrowOfEncodable
 
-lemma decode_list {β : Type _} [Encodable β] :
+lemma decode_list :
     (e : ℕ) → (decode e : Option (List β)) = (Denumerable.ofNat (List ℕ) e).mapM' (decode : ℕ → Option β)
   | 0     => by simp; rfl
   | e + 1 =>
     have : e.unpair.2 < e + 1 := Nat.lt_succ_of_le e.unpair_right_le
     by  simp; rcases h : (decode e.unpair.1 : Option β) with (_ | b) <;> simp[seq_eq_bind, Option.bind_eq_bind]
-        have := decode_list (β := β) (e.unpair.2)
+        have := decode_list (e.unpair.2)
         simp[this, Option.pure_eq_some, Option.map_eq_bind, Function.comp]
 
-lemma encodeDecode_list {β : Type _} [Encodable β] (e : ℕ) :
-    encodeDecode (List β) e = ((Denumerable.ofNat (List ℕ) e).mapM' (encodeDecode β : ℕ → Option ℕ)).map encode := by
-  simp[encodeDecode, decode_list]
-  generalize hr : (Denumerable.ofNat (List ℕ) e) = r
-  induction' r with rh rt ih generalizing e <;> simp[Option.pure_eq_some, Option.bind_eq_bind, Option.map_bind']
-  rcases hb : (decode rh) with (_ | b) <;> simp
-  rcases hbs : (mapM' decode rt) with (_ | bs) <;> simp
-  { have : mapM' (fun e => (encode (decode e : Option β)).predO) rt = none
-    { simp[encodeDecode, List.mapM'_eq_none_iff] at hbs ⊢
-      rcases hbs with ⟨a, ha, da⟩
-      exact ⟨a, ha, by simp[da]⟩  }
-    simp[this] }
-  { have ih : some (encode bs) = (mapM' (encodeDecode β) rt).map encode := by simpa[hbs] using ih (encode rt) (by simp)
-    suffices : some ((encode b).pair (encode bs) + 1) = ((mapM' (encodeDecode β) rt).map encode).map ((encode b).pair · + 1)
-    { simp[this]; simp[Option.map_eq_bind, Function.comp] }
-    simp[←ih] }
+lemma decode_vector (e : ℕ) :
+    (decode (α := Vector β k) e) = (decode (α := List β) e).bind (List.toVector k) := by
+  simp[decode, decodeSubtype, List.toVector]
 
-lemma encodeDecode_finArrow {β : Type _} [Encodable β] {e : ℕ} :
-    encodeDecode (Fin k → β) e =
-    (((Denumerable.ofNat (List ℕ) e).mapM' (encodeDecode β)).bind $ fun l' => if l'.length = k then some (encode l') else none) := by
-  rw[encodeDecode_ofEquiv, encodeDecode_subtype, encodeDecode_list]; simp
-  rcases h : (mapM' (encodeDecode β) (Denumerable.ofNat (List ℕ) e)) with (_ | l) <;> simp
-  rcases hbs : decode (encode l) with (_ | bs)
-  { simp[decode_list] at hbs
-    have : ∃ a ∈ l, (decode a : Option β) = none := by simpa[List.mapM'_eq_none_iff] using hbs
-    rcases this with ⟨a, hal, ha⟩
-    have : ∃ a', encodeDecode β a' = some a := List.mapM'_mem_inversion h hal
-    rcases this with ⟨a', ha'⟩
-    simpa [ha] using decode_encodeDecode ha' }
-  { have : bs.length = l.length := by
-      simp[decode_list] at hbs; exact List.length_mapM' hbs
-    simp[this] }
+lemma decode_fintypeArrow (ι : Type _) [Fintype ι] [Primcodable ι] [DecidableEq ι] (β : Type _) [Primcodable β] (e : ℕ) :
+    (decode (α := ι → β) e) = (decode (α := List β) e).bind (fun l => (l.toVector (Fintype.card ι)).map fintypeArrowEquivVector.symm) := by
+  simp[Primcodable.ofEquiv_toEncodable, Encodable.decode_ofEquiv]
+  rw[Encodable.decode_ofEquiv, decode_vector]; simp
+  rcases (decode e : Option (List β)) with (_ | bs) <;> simp; { rfl }
 
-lemma encodeDecode_fintypeArrow (α : Type _) (β : Type _) [DecidableEq α] [Fintype α] [Primcodable α] [Primcodable β] (e : ℕ) :
-    encodeDecode (α → β) e =
-    (((Denumerable.ofNat (List ℕ) e).mapM' (encodeDecode β)).bind $ fun l' => if l'.length = Fintype.card α then some (encode l') else none) := by
-  simp[Primcodable.ofEquiv_toEncodable, fintypeArrow]; rw[encodeDecode_ofEquiv]
-  exact encodeDecode_finArrow (β := β)
+lemma encode_list (l : List β) :
+    encode l = encode (l.map encode) := by induction l <;> simp[*]
+
+lemma encode_vector {n} (v : Vector β n) :
+    encode v = encode v.toList := Encodable.Subtype.encode_eq v
+
+lemma encode_finArrow {n} (f : Fin n → β) :
+    encode f = encode (List.ofFn f) := by simp[finArrow]; rw[Encodable.encode_ofEquiv, encode_vector]; simp
+
+lemma encode_fintypeArrow (ι : Type _) [Fintype ι] [Primcodable ι] [DecidableEq ι] (β : Type _) [Primcodable β] (f : ι → β) :
+    encode f = encode (fintypeArrowEquivFinArrow f) := by simp[Primcodable.ofEquiv_toEncodable]; rw[Encodable.encode_ofEquiv]
 
 end Encodable
 
@@ -315,128 +353,226 @@ namespace WType
 
 attribute [-instance] WType.instEncodableWType
 
-open Encodable Primrec
-variable {α : Type _} {β : α → Type _} [(a : α) → Fintype (β a)] [(a : α) → DecidableEq (β a)] [(a : α) → Primcodable (β a)] [Primcodable α] [Primrec.CardUniform β]
+open Encodable Primrec Primcodable UniformlyPrimcodable
+variable {α : Type _} {β : α → Type _}
+  [(a : α) → Fintype (β a)] [(a : α) → DecidableEq (β a)] [(a : α) → Primcodable (β a)] [Primcodable α] [PrimrecCard β]
 
-@[reducible]
-private def WType' {α : Type _} (β : α → Type _) [(a : α) → Fintype (β a)] [(a : α) → Primcodable (β a)] (n : ℕ) :=
-  { t : WType β // t.depth ≤ n }
+def elimOpt (γ : Type _) (fγ : (Σ a : α, β a → γ) → Option γ) : WType β → Option γ
+  | ⟨a, f⟩ => (toFinArrowOpt (fun b => elimOpt γ fγ (f b))).bind fun g => fγ ⟨a, g⟩
 
-def WType'.depth' : WType' β n → Fin (n + 1) := fun ⟨t, h⟩ => ⟨t.depth, Iff.mpr Nat.lt_succ h⟩
+@[reducible] def SubWType {α : Type _} (β : α → Type _)
+  [(a : α) → Fintype (β a)] [(a : α) → Primcodable (β a)] (n : ℕ) := { t : WType β // t.depth ≤ n }
 
-def WType'.equiv_zero : WType' β 0 ≃ Empty where
+namespace SubWType
+
+@[simp] lemma depth_le (t : SubWType β n) : t.val.depth ≤ n := t.property
+
+def elim' (γ : Type*) (fγ : (Σ a : α, β a → γ) → γ) (s) : SubWType β s → γ := fun ⟨t, _⟩ => t.elim γ fγ 
+
+lemma elim_const {w₁ : SubWType β s₁} {w₂ : SubWType β s₂} (h : w₁.val = w₂.val) (γ) (fγ : (Σ a : α, β a → γ) → γ) : 
+    elim' γ fγ s₁ w₁ = elim' γ fγ s₂ w₂ := by
+  rcases w₁ with ⟨w, hw₁⟩
+  rcases w₂ with ⟨w, hw₂⟩
+  simp at h; rcases h with rfl
+  simp[elim']
+
+def equiv_zero : SubWType β 0 ≃ Empty where
   toFun := fun ⟨x, h⟩ => False.elim (not_lt_of_ge h $ WType.depth_pos _)
   invFun := by rintro ⟨⟩
   left_inv := fun ⟨x, h⟩ => False.elim (not_lt_of_ge h $ WType.depth_pos _)
   right_inv := by rintro ⟨⟩
 
-def WType'.equiv_succ : WType' β (n + 1) ≃ (Σ a : α, β a → WType' β n) where
+def equiv_succ : SubWType β (n + 1) ≃ (Σ a : α, β a → SubWType β n) where
   toFun := fun ⟨t, h⟩ => by rcases t with ⟨a, f⟩; exact ⟨a, fun b => ⟨f b, by simp[WType.depth] at h; exact h b⟩⟩
-  invFun := fun ⟨a, f⟩ => ⟨WType.mk a (fun b => (f b).val), by simp[depth]; intro b; exact (f b).property⟩
+  invFun := fun ⟨a, f⟩ => ⟨WType.mk a (fun b => (f b).val), by simp[depth]⟩
   left_inv := fun ⟨t, h⟩ => by rcases t with ⟨a, f⟩; simp
   right_inv := fun ⟨a, f⟩ => by simp
 
-def WType'.primcodable_zero : Primcodable (WType' β 0) := Primcodable.ofEquiv _ WType'.equiv_zero
+def primcodable_zero : Primcodable (SubWType β 0) := Primcodable.ofEquiv _ equiv_zero
 
-def WType'.primcodable_succ (n) (i : Primcodable (WType' β n)) : Primcodable (WType' β (n + 1)) := Primcodable.ofEquiv _ WType'.equiv_succ
+def primcodable_succ (n) (i : Primcodable (SubWType β n)) : Primcodable (SubWType β (n + 1)) := Primcodable.ofEquiv _ equiv_succ
 
-instance WType'.primcodable (n : ℕ) : Primcodable (WType' β n) := Nat.rec WType'.primcodable_zero WType'.primcodable_succ n
-
---instance : Encodable (WType β) := by
---  haveI h' : ∀ n, Primcodable (WType' β n) := fun n => Nat.rec WType'.primcodable_zero WType'.primcodable_succ n
---  let f : WType β → Σ n, WType' β n := fun t => ⟨t.depth, ⟨t, le_rfl⟩⟩
---  let finv : (Σn, WType' β n) → WType β := fun p => p.2.1
---  have : ∀ t, finv (f t) = t := fun t => rfl
---  exact Encodable.ofLeftInverse f finv this
+instance _root_.Primcodable.SubWType (n : ℕ) : Primcodable (SubWType β n) := Nat.rec SubWType.primcodable_zero SubWType.primcodable_succ n
 
 attribute [-instance] Subtype.encodable Encodable.fintypeArrowOfEncodable
 
-lemma testeq {α : Type _} {a b c d : α} : a = b → b = c → c = d → a = d := by
-  intro hab hbc hcd; simp[hab, hbc, hcd]
+@[simp] lemma decode_zero : (decode e : Option (SubWType β 0)) = none := by
+  rcases (decode e) with (_ | w)
+  · rfl
+  · exact Empty.elim (equiv_zero w)
 
-lemma WType'.encodeDecode_EType' (s e) :
-    encodeDecode (WType' β s) e =
-    Nat.casesOn s (encodeDecode (WType' β 0) e)
-      (fun s => (decode e.unpair.1 : Option α).bind
-        $ fun a => (((Denumerable.ofNat (List ℕ) e.unpair.2).mapM' (encodeDecode (WType' β s))).bind
-          $ fun l => if l.length = Fintype.card (β a) then some (encode l) else none).map
-            $ fun b => (encode a).pair b) := by
-  rcases s with (_ | s)
-  · simp
-  · have := Encodable.decode_sigma_val (γ := fun a => β a → WType' β s) e
-    simp[WType'.primcodable, primcodable_succ, Primcodable.ofEquiv_toEncodable]
-    rw[encodeDecode_ofEquiv equiv_succ, encode_decode_sigma_s]
-    rcases ha : (decode e.unpair.1 : Option α) with (_ | a)
-    · simp
-    · simp[encode_decode_ofEquiv, encodeDecode_fintypeArrow (β a) (WType' β s)]
+lemma decode_succ :
+  (decode e : Option (SubWType β (s + 1))) =
+  ((decode e.unpair.1 : Option α).bind
+    $ fun a => (decode e.unpair.2 : Option (List (SubWType β s))).bind
+      $ fun l => (l.toVector (Fintype.card (β a))).map
+        $ fun v => ⟨⟨a, fun b => (fintypeArrowEquivVector.symm v b).val⟩, by simp[depth, Equiv.vectorEquivFin]⟩ ) := by
+  simp[Primcodable.SubWType, primcodable_succ, Primcodable.ofEquiv_toEncodable]
+  rw[Encodable.decode_ofEquiv equiv_succ, equiv_succ, Encodable.decode_sigma_val]
+  simp[Option.map_bind', Function.comp, Encodable.decode_ofEquiv]; congr
+  funext a
+  rw[decode_fintypeArrow]; simp[Option.map_bind']; congr
 
+section elimDecode
+
+variable {γ : Type _}
 variable (β)
 
-private def strongRecE {γ : Type _} [Encodable γ] (zero : ℕ → γ) (succ : α → List γ → Option γ) : ℕ × ℕ → List (Option γ) → Option γ := fun (s, e) ih =>
-  Nat.casesOn s (zero e)
-    (fun s => (decode e.unpair.1 : Option α).bind
-      $ fun a => (((Denumerable.ofNat (List ℕ) e.unpair.2).mapM' (fun c => ih.getI (s.pair c))).bind
-        $ fun l => if l.length = Fintype.card (β a) then some l else none).bind
-          $ fun v => succ a v)
-
-@[reducible]
-private def g : ℕ × ℕ → List (Option ℕ) → Option ℕ := fun (s, e) ih =>
-  Nat.casesOn s (encodeDecode (WType' β 0) e)
-    (fun s => (decode e.unpair.1 : Option α).bind
-      $ fun a => (((Denumerable.ofNat (List ℕ) e.unpair.2).mapM' (fun c => ih.getI (s.pair c))).bind
-        $ fun l => if l.length = Fintype.card (β a) then some (encode l) else none).map
-          $ fun v => (encode a).pair v)
+def elimDecode (f : α → List γ → γ) : ℕ → ℕ → Option γ :=
+ fun s e => (decode e : Option (SubWType β s)).map (elim' γ (fun ⟨a, v⟩ => f a (List.ofFn $ fintypeArrowEquivFinArrow v)) s)
 
 variable {β}
 
-private lemma gh : g β (s, e) ((List.range (s.pair e)).map (fun i => encodeDecode (WType' β i.unpair.1) i.unpair.2)) = encodeDecode (WType' β s) e := by
-  simp[WType'.encodeDecode_EType' s e, g]
-  rcases s with (_ | s) <;> simp
-  have :
-    mapM' (fun c =>
-            List.getI
-              (List.map (fun i => encodeDecode (WType.WType' β i.unpair.1) i.unpair.2) (List.range ((s + 1).pair e)))
-            (s.pair c))
-          (Denumerable.ofNat (List ℕ) e.unpair.2) =
-    mapM' (encodeDecode (WType.WType' β s)) (Denumerable.ofNat (List ℕ) e.unpair.2) :=
-    List.mapM'_eq_mapM'_of_eq _ (by
-      { intro c hc
-        have : s.pair c < (s + 1).pair e := by
-          have : c < e.unpair.2 := Denumerable.lt_of_mem_list _ _ hc
-          exact lt_of_lt_of_le (Nat.pair_lt_pair_right s this) (Nat.pair_le_pair_of_le (Nat.le_succ s) (Nat.unpair_right_le e))
-        simp[List.getI_map_range _ this]; rw[Nat.unpair_pair s c] })
+lemma elim'_eq_elimDecode [Inhabited γ] (f : (a : α) × (β a → γ) → γ) :
+    (decode e).map (elim' γ f s) = elimDecode β (fun a l => f ⟨a, fintypeArrowEquivFinArrow.symm (fun i => l.getI i)⟩) s e := by
+  simp[elimDecode]
+  rcases (decode e) with (_ | w) <;> simp
+  { congr; funext ⟨a, j⟩; simp; congr; funext b; simp }
+
+variable (β)
+
+lemma elimDecode_eq_induction (f : α → List γ → γ) (s e) :
+    elimDecode β f s e =
+    Nat.casesOn s none
+      (fun s => (decode e.unpair.1 : Option α).bind
+        $ fun a => (((Denumerable.ofNat (List ℕ) e.unpair.2).mapM' (elimDecode β f s)).bind
+          $ fun l => if l.length = Fintype.card (β a) then some l else none).map
+            $ fun v => f a v) := by
+  rcases s with (_ | s)
+  · simp[elimDecode]
+  · simp[elimDecode, SubWType.decode_succ, Option.map_bind', decode_list, Function.comp, List.mapM'_option_map]; congr
+    funext a
+    rcases hw : List.mapM' (decode : ℕ → Option (SubWType β s)) (Denumerable.ofNat (List ℕ) e.unpair.2) with (_ | w) <;> simp
+    { simp[List.toVector]
+      by_cases hlw : w.length = Fintype.card (β a) <;> simp[hlw, elim, elim']
+      { simp[Vector.get_mk_eq_get, List.ofFn_get_eq_map]; congr
+        rw[Encodable.fintypeArrowEquivFinArrow_fintypeEquivFin (fun i =>
+          WType.elim γ (fun x => f x.fst (List.ofFn (fintypeArrowEquivFinArrow x.snd))) (w.get (i.cast hlw.symm)).val)];
+        rw[List.ofFn_get_eq_map (fun z => WType.elim γ (fun x => f x.fst (List.ofFn (fintypeArrowEquivFinArrow x.snd))) z.val) w] } }
+
+
+@[reducible]
+private def elimDecodeG (f : α → List γ → γ) : ℕ × ℕ → List (Option γ) → Option γ := fun (s, e) ih =>
+  Nat.casesOn s none
+    (fun s => (decode e.unpair.1 : Option α).bind
+      $ fun a => (((Denumerable.ofNat (List ℕ) e.unpair.2).mapM' (fun c => ih.getI (s.pair c))).bind
+        $ fun l => if l.length = Fintype.card (β a) then some l else none).map
+          $ fun v => f a v)
+
+private lemma elimDecodeG_eq_elimDecode (f : α → List γ → γ) (s e) :
+    elimDecodeG β f (s, e) ((List.range (s.pair e)).map (fun i => elimDecode β f i.unpair.1 i.unpair.2)) = elimDecode β f s e := by
+  simp[elimDecode_eq_induction β f s e, elimDecodeG]
+  rcases s with (_ | s) <;> simp; congr
+  funext a
+  have : 
+    mapM' (fun c => ((List.range ((s + 1).pair e)).map $ fun i => elimDecode β f i.unpair.fst i.unpair.snd).getI (s.pair c))
+      (Denumerable.ofNat (List ℕ) e.unpair.2) =
+    mapM' (elimDecode β f s) (Denumerable.ofNat (List ℕ) e.unpair.2) :=
+  List.mapM'_eq_mapM'_of_eq _ (by
+  { intro c hc
+    have : s.pair c < (s + 1).pair e := by
+      have : c < e.unpair.2 := Denumerable.lt_of_mem_list _ _ hc
+      exact lt_of_lt_of_le (Nat.pair_lt_pair_right s this) (Nat.pair_le_pair_of_le (Nat.le_succ s) (Nat.unpair_right_le e))
+    simp[List.getI_map_range _ this] })
   rw[this]
 
-/-
--- 以下の証明はチェックに異常な時間がかかる（なぜ？）：
-example [Primcodable α] : Primrec₂ (fun a b => Nat.pair (Encodable.encode a.snd) b : (ℕ × ℕ × ℕ) × α → ℕ → ℕ) :=
-  Primrec₂.natPair.comp (Primrec.encode.comp (Primrec.snd.comp Primrec.fst)) Primrec.snd
+variable [Primcodable γ]
 
--- 以下はうまく行く
-example [Primcodable α] : Primrec₂ (fun a b => Nat.pair (Encodable.encode a.snd) b : (ℕ × ℕ × ℕ) × α → ℕ → ℕ) :=
-  by apply Primrec₂.natPair.comp (Primrec.encode.comp (Primrec.snd.comp Primrec.fst)) Primrec.snd
--/
+private lemma elimDecodeG_primrec {f : α → List γ → γ} (hf : Primrec₂ f) : Primrec₂ (elimDecodeG β f) :=
+  by apply Primrec.nat_casesOn (fst.comp fst) (const none)
+      (by apply option_bind (Primrec.decode.comp $ fst.comp $ Primrec.unpair.comp $ snd.comp $ fst.comp fst)
+            (by apply option_map
+                  (option_bind
+                    (by apply option_list_mapM'
+                          (by apply (Primrec.ofNat _).comp $
+                                snd.comp $ Primrec.unpair.comp $ snd.comp $ fst.comp $ fst.comp $ fst)
+                          (by apply Primrec.list_getI.comp
+                                (snd.comp $ fst.comp $ fst.comp $ fst)
+                                (Primrec₂.natPair.comp (snd.comp $ fst.comp fst) snd)))
+                    (by apply Primrec.ite
+                          (Primrec.eq.comp (list_length.comp snd) (PrimrecCard.card_prim.comp $ snd.comp fst))
+                          (option_some.comp snd)
+                          (const none)))
+                  (hf.comp₂ (snd.comp₂ Primrec₂.left) Primrec₂.right)))
 
-private lemma g_primrec : Primrec₂ (g β) :=
-  have h₁ : Primrec₂ (fun a b => Nat.pair (encode a.snd) b : (((ℕ × ℕ) × List (Option ℕ)) × ℕ) × α → ℕ → ℕ) := by 
-    apply Primrec₂.natPair.comp (Primrec.encode.comp (snd.comp fst)) snd
-  have h₂ : Primrec₂ (fun a l => if l.length = Fintype.card (β a.snd) then some (encode l) else none
-    : (((ℕ × ℕ) × List (Option ℕ)) × ℕ) × α → List ℕ → Option ℕ) := by
-    apply Primrec.ite (Primrec.eq.comp (list_length.comp snd) (CardUniform.card_prim.comp $ snd.comp fst))
-      (Primrec.option_some.comp $ Primrec.encode.comp snd) (const none)
-  have h₃ : Primrec (fun a => mapM' (fun c => a.1.1.2.getI (a.1.2.pair c)) (Denumerable.ofNat (List ℕ) a.1.1.1.2.unpair.2)
-    : (((ℕ × ℕ) × List (Option ℕ)) × ℕ) × α → Option (List ℕ)) := by
-    apply option_list_mapM'
-      (by apply (Primrec.ofNat _).comp $ snd.comp $ Primrec.unpair.comp $ snd.comp $ fst.comp $ fst.comp $ fst)
-      (by apply Primrec.list_getI.comp (snd.comp $ fst.comp $ fst.comp $ fst) (Primrec₂.natPair.comp (snd.comp $ fst.comp fst) snd))
-  by apply Primrec.nat_casesOn (fst.comp fst) (Primrec.encodeDecode.comp (snd.comp fst))
-      (by apply
-            Primrec.option_bind (Primrec.decode.comp $ fst.comp $ Primrec.unpair.comp $ snd.comp $ fst.comp fst)
-            (by apply Primrec.option_map (by apply Primrec.option_bind (by apply h₃) (by apply h₂)) h₁))
+lemma primrec_elimDecode {f : α → List γ → γ} (hf : Primrec₂ f) : Primrec₂ (elimDecode β f) := by
+  have : Primrec₂ (fun p t => some (elimDecodeG β f p t)) := option_some.comp (elimDecodeG_primrec β hf)
+  exact nat_strong_rec'2' _ this (by simp[elimDecodeG_eq_elimDecode β f])
 
-lemma WType'.uniform : Primrec.Uniform (WType' β) :=
-  have : Primrec₂ (fun p t => some (g β p t)) := option_some.comp g_primrec
-  Uniform.ofEncodeDecode (nat_strong_rec'2' _ this (by simp[gh]))
+end elimDecode
+
+lemma encode_eq_elim' : ∀ w : SubWType β s, encode w = elim' ℕ encode s w := by
+  { induction' s with s ih
+    · simp; intro w h; simpa using lt_of_lt_of_le (depth_pos w) h
+    · rintro ⟨⟨a, f⟩, hw⟩; simp[elim', elim, Primcodable.SubWType, primcodable_succ, Primcodable.ofEquiv_toEncodable]
+      rw[Encodable.encode_ofEquiv equiv_succ]
+      simp[equiv_succ, Encodable.encode_sigma_val]
+      rw[Encodable.encode_sigma_val, Encodable.encode_sigma_val, encode_fintypeArrow, encode_finArrow, encode_list]
+      simp[Function.comp]; rw[←encode_finArrow, encode_fintypeArrow (β a)]; simp
+      congr; funext i; simp; rw[ih]; rfl }
+
+lemma encodeDecode_eq_elimDecode (s e : ℕ) : encodeDecode (SubWType β s) e = elimDecode β (fun a l => encode (a, l)) s e := by
+  simp[elimDecode, encodeDecode_eq_encode_map_decode]
+  rcases (decode e) <;> simp[encode_eq_elim']; congr
+  funext ⟨a, f⟩; simp[encode_fintypeArrow, encode_finArrow]
+
+instance uniformlyPrimcodable : UniformlyPrimcodable (SubWType β) :=
+  UniformlyPrimcodable.ofEncodeDecode (by
+    have : Primrec₂ (elimDecode β (fun a l => encode (a, l))) :=
+      primrec_elimDecode β (Primrec.encode.comp $ Primrec₂.pair.comp fst snd)
+    exact this.of_eq (by simp[encodeDecode_eq_elimDecode]))
+
+lemma depth_eq_elimDecode (s e : ℕ) :
+    (decode e : Option (SubWType β s)).map (fun w => w.val.depth) = elimDecode β (fun a l => l.sup + 1) s e := by
+  have : ∀ w : SubWType β s, depth w.val = elim' ℕ (fun p => Finset.sup Finset.univ p.snd + 1) s w
+  { induction' s with s ih
+    · simp; intro w h; simpa using lt_of_lt_of_le (depth_pos w) h
+    · rintro ⟨⟨a, f⟩, hw⟩;
+      simp[depth, ih, elim', elim]
+      have : ∀ (b : β a), depth (f b) = elim ℕ (fun p => Finset.sup Finset.univ p.snd + 1) (f b) :=
+        fun b => ih ⟨f b, by simp[depth, Nat.succ_eq_add_one] at hw; exact hw b⟩
+      simp[this] }
+  simp[elimDecode, encodeDecode_eq_encode_map_decode]
+  rcases (decode e) <;> simp[this]; congr
+  funext ⟨a, f⟩; simp[List.sup_ofFn, fintypeArrowEquivFinArrow_eq]
+
+lemma depth_decode_primrec : Primrec₂ (fun s e => (decode e : Option (SubWType β s)).map (fun w => w.val.depth)) := by
+  have : Primrec₂ (elimDecode β (fun a l => l.sup + 1)) :=
+    primrec_elimDecode β (by simp[←Nat.succ_eq_add_one]; apply Primrec.succ.comp $ (list_sup nat_max).comp snd)
+  exact this.of_eq (by simp[depth_eq_elimDecode])
+
+def ofW : WType β → (s : ℕ) × SubWType β s := fun w => ⟨w.depth, ⟨w, by rfl⟩⟩
+
+def toW : (s : ℕ) × SubWType β s → WType β := fun ⟨_, w⟩ => w
+
+end SubWType
+
+private lemma encode_decode_eq (e : ℕ) :
+    Option.casesOn ((decode e : Option ((s : ℕ) × SubWType β s)).map SubWType.toW) 0 (fun w => encode (SubWType.ofW w) + 1) =
+    encode (((encodeDecode (SubWType β e.unpair.1) e.unpair.2).bind
+      $ fun c => ((decode c : Option (SubWType β e.unpair.1)).map (fun w => w.val.depth)).map
+        $ fun d => d.pair c)) := by
+  simp[Function.comp, encodeDecode_eq_encode_map_decode]
+  rcases (decode e.unpair.2) with (_ | w) <;> simp[SubWType.toW, SubWType.ofW]
+  { simp[SubWType.encode_eq_elim']; apply SubWType.elim_const; simp }
+
+private lemma primrec_encode_decode :
+    Primrec (fun e => 
+      encode (((encodeDecode (SubWType β e.unpair.1) e.unpair.2).bind
+        $ fun c => ((decode c : Option (SubWType β e.unpair.1)).map (fun w => w.val.depth)).map
+          $ fun d => d.pair c)) : ℕ → ℕ) :=
+  (Primrec.encode.comp $
+    option_bind (Primrec₂.encodeDecode_u.comp (fst.comp Primrec.unpair) (snd.comp Primrec.unpair))
+      (option_map (SubWType.depth_decode_primrec.comp (fst.comp $ Primrec.unpair.comp fst) snd)
+        (Primrec₂.natPair.comp₂ Primrec₂.right (snd.comp fst))))
+
+private def encodable : Encodable (WType β) where
+  encode := fun w => encode (SubWType.ofW w)
+  decode := fun e => (decode e).map SubWType.toW
+  encodek := by rintro ⟨a, f⟩; simp[SubWType.toW, SubWType.ofW]
+
+instance _root_.Primcodable.wtype : Primcodable (WType β) :=
+  { encodable with
+    prim := Primrec.nat_iff.mp <| primrec_encode_decode.of_eq (fun e => (encode_decode_eq e).symm) }
 
 end WType
-
